proof/iu_system/uni/decl_worklist/def.v
@@ -115,15 +115,15 @@ Inductive d_wl_red : dworklist -> Prop :=    (* defn d_wl_red *)
  | d_wl_red__tvar : forall (Ω:dworklist) (X:atom),
     d_wl_red Ω ->
     d_wl_red (dworklist_constvar Ω X dbind_tvar_empty)
- | d_wl_red__stvar : forall (Ω:dworklist) (SX:atom),
+ | d_wl_red__stvar : forall (Ω:dworklist) (X:atom),
     d_wl_red Ω ->
-    d_wl_red (dworklist_constvar Ω SX dbind_stvar_empty)
- | d_wl_red__subtop : forall (Ω:dworklist) (A1:typ),
+    d_wl_red (dworklist_constvar Ω X dbind_stvar_empty)
+ | d_wl_red__subtop : forall (Ω:dworklist) (A:typ),
      d_wl_red Ω ->
-     d_wl_red (dworklist_conswork Ω (work_sub A1 typ_top))
- | d_wl_red__sub_bot : forall (Ω:dworklist) (A1:typ),
+     d_wl_red (dworklist_conswork Ω (work_sub A typ_top))
+ | d_wl_red__sub_bot : forall (Ω:dworklist) (B:typ),
      d_wl_red Ω ->
-     d_wl_red (dworklist_conswork Ω (work_sub typ_bot A1))
+     d_wl_red (dworklist_conswork Ω (work_sub typ_bot B))
  | d_wl_red__sub_unit : forall (Ω:dworklist),
      d_wl_red Ω ->
      d_wl_red (dworklist_conswork Ω (work_sub typ_unit typ_unit))
@@ -133,37 +133,37 @@ Inductive d_wl_red : dworklist -> Prop :=    (* defn d_wl_red *)
  | d_wl_red__subarrow : forall (Ω:dworklist) (A1 A2 B1 B2:typ),
      d_wl_red (dworklist_conswork (dworklist_conswork Ω (work_sub B1 A1)) (work_sub A2 B2)) ->
      d_wl_red (dworklist_conswork Ω (work_sub (typ_arrow A1 A2) (typ_arrow B1 B2)))
- | d_wl_red__sub_all : forall (L:vars) (Ω:dworklist) (A1 B1:typ),
-     ( forall X , X `notin` L -> d_wl_red (dworklist_conswork (dworklist_constvar Ω X dbind_stvar_empty) (work_sub  (open_typ_wrt_typ  A1   (typ_var_f X) )   (open_typ_wrt_typ  B1   (typ_var_f X) ) ))) ->
-     d_wl_red (dworklist_conswork Ω (work_sub (typ_all A1) (typ_all B1)))    
- | d_wl_red__sub_alll : forall (Ω:dworklist) (A1 B1 T1:typ),
-     neq_all B1 ->
-     neq_intersection B1 ->
-     neq_union B1 -> 
-     d_mono_typ ( dwl_to_denv  Ω  )  T1 ->
-     d_wl_red (dworklist_conswork Ω (work_sub  (open_typ_wrt_typ  A1   T1 )  B1)) ->
-     d_wl_red (dworklist_conswork Ω (work_sub (typ_all A1) B1))
- | d_wl_red__sub_intersection1 : forall (Ω:dworklist) (A1 B1 B2:typ),
-     d_wl_red (dworklist_conswork (dworklist_conswork Ω (work_sub A1 B1)) (work_sub A1 B2)) ->
-     d_wl_red (dworklist_conswork Ω (work_sub A1 (typ_intersection B1 B2)))
- | d_wl_red__sub_intersection2 : forall (Ω:dworklist) (A1 A2 B1:typ),
-     d_wl_red (dworklist_conswork Ω (work_sub A1 B1)) ->
-     d_wl_red (dworklist_conswork Ω (work_sub (typ_intersection A1 A2) B1))
- | d_wl_red__sub_intersection3 : forall (Ω:dworklist) (A1 A2 B1:typ),
-     d_wl_red (dworklist_conswork Ω (work_sub A2 B1)) ->
-     d_wl_red (dworklist_conswork Ω (work_sub (typ_intersection A1 A2) B1))
- | d_wl_red__sub_union1 : forall (Ω:dworklist) (A1 B1 B2:typ),
-     d_wl_red (dworklist_conswork Ω (work_sub A1 B1)) ->
-     d_wl_red (dworklist_conswork Ω (work_sub A1 (typ_union B1 B2)))
- | d_wl_red__sub_union2 : forall (Ω:dworklist) (A1 B1 B2:typ),
-     d_wl_red (dworklist_conswork Ω (work_sub A1 B2)) ->
-     d_wl_red (dworklist_conswork Ω (work_sub A1 (typ_union B1 B2)))
+ | d_wl_red__sub_all : forall (L:vars) (Ω:dworklist) (A B:typ),
+     ( forall X , X `notin` L -> d_wl_red (dworklist_conswork (dworklist_constvar Ω X dbind_stvar_empty) (work_sub  (open_typ_wrt_typ  A   (typ_var_f X) )   (open_typ_wrt_typ  B   (typ_var_f X) ) ))) ->
+     d_wl_red (dworklist_conswork Ω (work_sub (typ_all A) (typ_all B)))    
+ | d_wl_red__sub_alll : forall (Ω:dworklist) (A B T:typ),
+     neq_all B ->
+     neq_intersection B ->
+     neq_union B -> 
+     d_mono_typ ( dwl_to_denv  Ω  )  T ->
+     d_wl_red (dworklist_conswork Ω (work_sub  (open_typ_wrt_typ  A   T )  B)) ->
+     d_wl_red (dworklist_conswork Ω (work_sub (typ_all A) B))
+ | d_wl_red__sub_intersection1 : forall (Ω:dworklist) (A B1 B2:typ),
+     d_wl_red (dworklist_conswork (dworklist_conswork Ω (work_sub A B1)) (work_sub A B2)) ->
+     d_wl_red (dworklist_conswork Ω (work_sub A (typ_intersection B1 B2)))
+ | d_wl_red__sub_intersection2 : forall (Ω:dworklist) (A1 A2 B:typ),
+     d_wl_red (dworklist_conswork Ω (work_sub A1 B)) ->
+     d_wl_red (dworklist_conswork Ω (work_sub (typ_intersection A1 A2) B))
+ | d_wl_red__sub_intersection3 : forall (Ω:dworklist) (A1 A2 B:typ),
+     d_wl_red (dworklist_conswork Ω (work_sub A2 B)) ->
+     d_wl_red (dworklist_conswork Ω (work_sub (typ_intersection A1 A2) B))
+ | d_wl_red__sub_union1 : forall (Ω:dworklist) (A B1 B2:typ),
+     d_wl_red (dworklist_conswork Ω (work_sub A B1)) ->
+     d_wl_red (dworklist_conswork Ω (work_sub A (typ_union B1 B2)))
+ | d_wl_red__sub_union2 : forall (Ω:dworklist) (A B1 B2:typ),
+     d_wl_red (dworklist_conswork Ω (work_sub A B2)) ->
+     d_wl_red (dworklist_conswork Ω (work_sub A (typ_union B1 B2)))
  | d_wl_red__sub_union3 : forall (Ω:dworklist) (A1 A2 B1:typ),
      d_wl_red (dworklist_conswork (dworklist_conswork Ω (work_sub A1 B1)) (work_sub A2 B1)) ->
      d_wl_red (dworklist_conswork Ω (work_sub (typ_union A1 A2) B1))
- | d_wl_red__chk_sub : forall (Ω:dworklist) (e:exp) (A1:typ),
-     d_wl_red (dworklist_conswork Ω (work_infer e (cont_sub A1))) ->
-     d_wl_red (dworklist_conswork Ω (work_check e A1))
+ | d_wl_red__chk_sub : forall (Ω:dworklist) (e:exp) (A:typ),
+     d_wl_red (dworklist_conswork Ω (work_infer e (cont_sub A))) ->
+     d_wl_red (dworklist_conswork Ω (work_check e A))
  (* | d_wl_red__chkall : forall (L:vars) (Ω:dworklist) (e:exp) (T1:typ),
       ( forall X , X \notin  L  -> ds_in X  ( open_typ_wrt_typ T1 (typ_var_f X) )  )  ->
       ( forall X , X \notin  L  -> d_wl_red (dworklist_conswork (dworklist_constvar Ω X dbind_tvar_empty) (work_check e  ( open_typ_wrt_typ T1 (typ_var_f X) ) )) )  ->
@@ -183,57 +183,57 @@ Inductive d_wl_red : dworklist -> Prop :=    (* defn d_wl_red *)
  | d_wl_red__chk_union2 : forall (Ω:dworklist) (e:exp) (A1 A2:typ),
      d_wl_red (dworklist_conswork Ω (work_check e A2)) ->
      d_wl_red (dworklist_conswork Ω (work_check e (typ_union A1 A2)))
- | d_wl_red__inf_var : forall (Ω:dworklist) (x:expvar) (c:cont) (A1:typ),
-      binds ( x )  ( (dbind_typ A1) ) (  ( dwl_to_denv  Ω  )  )  ->
-     d_wl_red (dworklist_conswork Ω (work_apply c A1)) ->
+ | d_wl_red__inf_var : forall (Ω:dworklist) (x:expvar) (c:cont) (A:typ),
+      binds ( x )  ( (dbind_typ A) ) (  ( dwl_to_denv  Ω  )  )  ->
+     d_wl_red (dworklist_conswork Ω (work_apply c A)) ->
      d_wl_red (dworklist_conswork Ω (work_infer (exp_var_f x) c))
- | d_wl_red__inf_anno : forall (Ω:dworklist) (e:exp) (A1:typ) (c:cont),
-     d_wl_red (dworklist_conswork (dworklist_conswork Ω (work_apply c  A1)) (work_check e A1)) ->
-     d_wl_red (dworklist_conswork Ω (work_infer  ( (exp_anno e A1) )  c))
- | d_wl_red__inf_tabs : forall (L:vars) (Ω:dworklist) (e:exp) (A1:typ) (c:cont),
+ | d_wl_red__inf_anno : forall (Ω:dworklist) (e:exp) (A:typ) (c:cont),
+     d_wl_red (dworklist_conswork (dworklist_conswork Ω (work_apply c  A)) (work_check e A)) ->
+     d_wl_red (dworklist_conswork Ω (work_infer  ( (exp_anno e A) )  c))
+ | d_wl_red__inf_tabs : forall (L:vars) (Ω:dworklist) (e:exp) (A:typ) (c:cont),
       (* ( forall X , X \notin  L  -> ds_in X  ( open_typ_wrt_typ A1 (typ_var_f X) )  )  -> *)
-      ( forall X , X \notin  L  -> d_wl_red (dworklist_conswork (dworklist_constvar (dworklist_conswork Ω (work_apply c  (typ_all A1) )) X dbind_tvar_empty) (work_check (exp_anno  ( open_exp_wrt_typ e (typ_var_f X) ) ( open_typ_wrt_typ A1 (typ_var_f X) ) )  ( open_typ_wrt_typ A1 (typ_var_f X) ) )) )  ->
-     d_wl_red (dworklist_conswork Ω (work_infer (exp_tabs (body_anno e A1)) c))
+      ( forall X , X \notin  L  -> d_wl_red (dworklist_conswork (dworklist_constvar (dworklist_conswork Ω (work_apply c  (typ_all A) )) X dbind_tvar_empty) (work_check (exp_anno  ( open_exp_wrt_typ e (typ_var_f X) ) ( open_typ_wrt_typ A (typ_var_f X) ) )  ( open_typ_wrt_typ A (typ_var_f X) ) )) )  ->
+     d_wl_red (dworklist_conswork Ω (work_infer (exp_tabs (body_anno e A)) c))
  | d_wl_red__inf_unit : forall (Ω:dworklist) (c:cont),
      d_wl_red (dworklist_conswork Ω (work_apply c typ_unit)) ->
      d_wl_red (dworklist_conswork Ω (work_infer exp_unit c))
  | d_wl_red__inf_app : forall (Ω:dworklist) (e1 e2:exp) (c:cont),
      d_wl_red (dworklist_conswork Ω (work_infer e1 (cont_infabs (cont_infapp e2 c)))) ->
      d_wl_red (dworklist_conswork Ω (work_infer  ( (exp_app e1 e2) )  c))
- | d_wl_red__inf_tapp : forall (Ω:dworklist) (e:exp) (T:typ) (c:cont),
-     d_wl_red (dworklist_conswork Ω (work_infer e (cont_inftapp T c))) ->
-     d_wl_red (dworklist_conswork Ω (work_infer (exp_tapp e T) c))
- | d_wl_red__inftapp_all : forall (Ω:dworklist) (T1 T2:typ) (c:cont),
-     d_wl_red (dworklist_conswork Ω (work_apply c (open_typ_wrt_typ  T1   T2 ) )) ->
-     d_wl_red (dworklist_conswork Ω (work_inftapp (typ_all T1) T2 c))
- | d_wl_red__inftapp_bot : forall (Ω:dworklist) (T:typ) (c:cont),
+ | d_wl_red__inf_tapp : forall (Ω:dworklist) (e:exp) (B:typ) (c:cont),
+     d_wl_red (dworklist_conswork Ω (work_infer e (cont_inftapp B c))) ->
+     d_wl_red (dworklist_conswork Ω (work_infer (exp_tapp e B) c))
+ | d_wl_red__inftapp_all : forall (Ω:dworklist) (A B:typ) (c:cont),
+     d_wl_red (dworklist_conswork Ω (work_apply c (open_typ_wrt_typ  A   B ) )) ->
+     d_wl_red (dworklist_conswork Ω (work_inftapp (typ_all A) B c))
+ | d_wl_red__inftapp_bot : forall (Ω:dworklist) (B:typ) (c:cont),
      d_wl_red (dworklist_conswork Ω (work_apply c typ_bot)) ->
-     d_wl_red (dworklist_conswork Ω (work_inftapp typ_bot T c))
- | d_wl_red__inftapp_inter1 : forall (Ω:dworklist) (A1 A2 B1:typ) (c:cont),
-     d_wl_red (dworklist_conswork Ω (work_inftapp A1 B1 c)) ->
-     d_wl_red (dworklist_conswork Ω (work_inftapp (typ_intersection A1 A2) B1 c))
- | d_wl_red__inftapp_inter2: forall (Ω:dworklist) (A1 A2 B1:typ) (c:cont),
-     d_wl_red (dworklist_conswork Ω (work_inftapp A2 B1 c)) ->
-     d_wl_red (dworklist_conswork Ω (work_inftapp (typ_intersection A1 A2) B1 c))
- | d_wl_red__inftapp_union : forall (Ω:dworklist) (A1 A2 B1:typ) (c:cont),
-     d_wl_red (dworklist_conswork Ω (work_inftapp A1 B1 (cont_inftappunion A2 B1 c))) ->
-     d_wl_red (dworklist_conswork Ω (work_inftapp (typ_union A1 A2) B1 c))
- | d_wl_red__inftappunion : forall (Ω:dworklist) (A2 B2 C1:typ) (c:cont),
-     d_wl_red (dworklist_conswork Ω (work_inftapp A2 B2 (cont_unioninftapp C1 c) ))->
-     d_wl_red (dworklist_conswork Ω (work_inftappunion C1 A2 B2 c))
+     d_wl_red (dworklist_conswork Ω (work_inftapp typ_bot B c))
+ | d_wl_red__inftapp_inter1 : forall (Ω:dworklist) (A1 A2 B:typ) (c:cont),
+     d_wl_red (dworklist_conswork Ω (work_inftapp A1 B c)) ->
+     d_wl_red (dworklist_conswork Ω (work_inftapp (typ_intersection A1 A2) B c))
+ | d_wl_red__inftapp_inter2: forall (Ω:dworklist) (A1 A2 B:typ) (c:cont),
+     d_wl_red (dworklist_conswork Ω (work_inftapp A2 B c)) ->
+     d_wl_red (dworklist_conswork Ω (work_inftapp (typ_intersection A1 A2) B c))
+ | d_wl_red__inftapp_union : forall (Ω:dworklist) (A1 A2 B:typ) (c:cont),
+     d_wl_red (dworklist_conswork Ω (work_inftapp A1 B (cont_inftappunion A2 B c))) ->
+     d_wl_red (dworklist_conswork Ω (work_inftapp (typ_union A1 A2) B c))
+ | d_wl_red__inftappunion : forall (Ω:dworklist) (A B C:typ) (c:cont),
+     d_wl_red (dworklist_conswork Ω (work_inftapp A B (cont_unioninftapp C c) ))->
+     d_wl_red (dworklist_conswork Ω (work_inftappunion C A B c))
  | d_wl_red__unioninftapp : forall (Ω:dworklist) (A1 A2:typ) (c:cont),
      d_wl_red (dworklist_conswork Ω (work_apply c (typ_union A1 A2)))->
      d_wl_red (dworklist_conswork Ω (work_unioninftapp A1 A2 c))
- | d_wl_red__infabs_arrow : forall (Ω:dworklist) (T1 T2:typ) (c:cont),
-     d_wl_red (dworklist_conswork Ω (work_apply c (typ_arrow T1 T2))) ->
-     d_wl_red (dworklist_conswork Ω (work_infabs (typ_arrow T1 T2) c))
+ | d_wl_red__infabs_arrow : forall (Ω:dworklist) (A B:typ) (c:cont),
+     d_wl_red (dworklist_conswork Ω (work_apply c (typ_arrow A B))) ->
+     d_wl_red (dworklist_conswork Ω (work_infabs (typ_arrow A B) c))
  | d_wl_red__infabs_bot : forall (Ω:dworklist) (c:cont),
      d_wl_red (dworklist_conswork Ω (work_apply c (typ_arrow typ_top typ_bot))) ->
      d_wl_red (dworklist_conswork Ω (work_infabs typ_bot c))
- | d_wl_red__infabs_all : forall (Ω:dworklist) (A1 T1:typ) (c:cont),
-     d_mono_typ (dwl_to_denv Ω) T1 ->
-     d_wl_red (dworklist_conswork Ω (work_infabs (open_typ_wrt_typ A1 T1) c)) ->
-     d_wl_red (dworklist_conswork Ω (work_infabs (typ_all A1) c))
+ | d_wl_red__infabs_all : forall (Ω:dworklist) (A T:typ) (c:cont),
+     d_mono_typ (dwl_to_denv Ω) T ->
+     d_wl_red (dworklist_conswork Ω (work_infabs (open_typ_wrt_typ A T) c)) ->
+     d_wl_red (dworklist_conswork Ω (work_infabs (typ_all A) c))
  | d_wl_red__infabs_inter1 : forall (Ω:dworklist) (A1 A2:typ) (c:cont),
      d_wl_red (dworklist_conswork Ω (work_infabs A1 c)) ->
      d_wl_red (dworklist_conswork Ω (work_infabs (typ_intersection A1 A2) c))
@@ -246,16 +246,16 @@ Inductive d_wl_red : dworklist -> Prop :=    (* defn d_wl_red *)
  | d_wl_red__unioninfabs: forall (Ω:dworklist) (A1 A2 B1 B2:typ) (c:cont),
      d_wl_red (dworklist_conswork Ω (work_apply c (typ_arrow (typ_intersection A1 A2) (typ_union B1 B2)))) ->
      d_wl_red (dworklist_conswork Ω (work_unioninfabs (typ_arrow A1 B1) (typ_arrow A2 B2) c))
- | d_wl_red__infabsunion: forall (Ω:dworklist) (A2 B1 C1:typ) (c:cont),
-     d_wl_red (dworklist_conswork Ω (work_infabs A2 (cont_unioninfabs (typ_arrow B1 C1) c))) ->
-     d_wl_red (dworklist_conswork Ω (work_infabsunion (typ_arrow B1 C1) A2 c))
- | d_wl_red__infapp: forall (Ω:dworklist) (e:exp) (A1 B1:typ) (c:cont),
-     d_wl_red (dworklist_conswork (dworklist_conswork Ω (work_check e A1)) (work_apply c B1)) ->
-     d_wl_red (dworklist_conswork Ω (work_infapp (typ_arrow A1 B1) e c))
- | d_wl_red__applycont : forall (Ω:dworklist) (w:work) (T1:typ) (c:cont),
-     apply_cont c T1 w ->
+ | d_wl_red__infabsunion: forall (Ω:dworklist) (A B C:typ) (c:cont),
+     d_wl_red (dworklist_conswork Ω (work_infabs A (cont_unioninfabs (typ_arrow B C) c))) ->
+     d_wl_red (dworklist_conswork Ω (work_infabsunion (typ_arrow B C) A c))
+ | d_wl_red__infapp: forall (Ω:dworklist) (e:exp) (A B:typ) (c:cont),
+     d_wl_red (dworklist_conswork (dworklist_conswork Ω (work_check e A)) (work_apply c B)) ->
+     d_wl_red (dworklist_conswork Ω (work_infapp (typ_arrow A B) e c))
+ | d_wl_red__applycont : forall (Ω:dworklist) (w:work) (A:typ) (c:cont),
+     apply_cont c A w ->
      d_wl_red (dworklist_conswork Ω w) ->
-     d_wl_red (dworklist_conswork Ω (work_apply c T1))   
+     d_wl_red (dworklist_conswork Ω (work_apply c A))   
     .
 
 
